freevars.lean
@@ -1220,3 +1220,34 @@ lemma vc.closed.implies.inv {P Q: vc}: closed (vc.implies P Q) → closed P ∧ 
   have P_closed: closed P, from vc.closed.not.inv P_not_closed,
   have Q_closed: closed Q, from (vc.closed.or.inv P_not_or_Q_closed).right,
   ⟨P_closed, Q_closed⟩
+
+lemma same_free_and_left {P P' Q: prop}: FV P' = FV P → (FV (P' ⋀ Q) = FV (P ⋀ Q)) :=
+  assume free_P'_P: FV P' = FV P,
+  set.eq_of_subset_of_subset (
+    assume x,
+    assume : x ∈ FV (P' ⋀ Q),
+    or.elim (free_in_prop.and.inv this) (
+      assume : x ∈ FV P',
+      have x ∈ FV P, from free_P'_P ▸ this,
+      show x ∈ FV (P ⋀ Q), from free_in_prop.and₁ this
+    ) (
+      assume : x ∈ FV Q,
+      show x ∈ FV (P ⋀ Q), from free_in_prop.and₂ this
+    )
+  ) (
+    assume x,
+    assume : x ∈ FV (P ⋀ Q),
+    or.elim (free_in_prop.and.inv this) (
+      assume : x ∈ FV P,
+      have x ∈ FV P', from free_P'_P.symm ▸ this,
+      show x ∈ FV (P' ⋀ Q), from free_in_prop.and₁ this
+    ) (
+      assume : x ∈ FV Q,
+      show x ∈ FV (P' ⋀ Q), from free_in_prop.and₂ this
+    )
+  )
+
+lemma free_in_left {P Q: prop}: FV P ⊆ FV (P ⋀ Q) :=
+  assume x: var,
+  assume : x ∈ FV P,
+  show x ∈ FV (P ⋀ Q), from free_in_prop.and₁ this
